Partial first try at interoperating with buffers of UInt32

vale/code/arch/x64/Interop.fst
@@ -12,6 +12,8 @@ open X64.Machine_s
 open X64.Bytes_Semantics_s
 open X64.Bytes_Semantics
 
+open Views
+
 friend SecretByte
 
 #reset-options "--max_fuel 2 --initial_fuel 2 --max_ifuel 1 --initial_ifuel 1"
@@ -22,167 +24,29 @@ friend SecretByte
 assume val ref_extensionality (#a:Type0) (#rel:Preorder.preorder a) (h:Heap.heap) (r1 r2:Heap.mref a rel) : Lemma 
   (Heap.contains h r1 /\ Heap.contains h r2 /\ Heap.addr_of r1 = Heap.addr_of r2 ==> r1 == r2)
 
-
-(* Write a buffer in the vale memory *)
-
-let rec write_vale_mem (contents:Seq.seq UInt8.t) (length:nat{length = FStar.Seq.Base.length contents}) addr (i:nat{i <= length}) 
-      (curr_heap:heap{forall j. {:pattern (Seq.index contents j)} 
-	0 <= j /\ j < i ==> curr_heap.[addr+j] == UInt8.v (Seq.index contents j)}) : Tot heap (decreases %[sub length i]) =
-    if i >= length then curr_heap
-    else (
-      let heap = curr_heap.[addr + i] <- UInt8.v (FStar.Seq.index contents i) in
-      write_vale_mem contents length addr (i+1) heap
-    )      
-
-let rec frame_write_vale_mem (contents:Seq.seq UInt8.t) (length:nat{length = FStar.Seq.Base.length contents}) addr (i:nat{i <= length}) 
-      (curr_heap:heap{forall j. {:pattern (Seq.index contents j)} 0 <= j /\ j < i ==> curr_heap.[addr + j] == UInt8.v (Seq.index contents j)}) : Lemma
-      (requires True)
-      (ensures (let new_heap = write_vale_mem contents length addr i curr_heap in
-      forall j. j < addr \/ j >= addr + length ==> curr_heap.[j] == new_heap.[j]))
-      (decreases %[sub length i])=
-      if i >= length then ()
-      else begin
-	let heap = curr_heap.[addr + i] <- UInt8.v (FStar.Seq.index contents i) in
-	frame_write_vale_mem contents length addr (i+1) heap
-      end
-      
-let rec load_store_write_vale_mem 
-  (contents:Seq.seq UInt8.t) 
-  (length:nat{length = FStar.Seq.Base.length contents}) 
-  addr 
-  (i:nat{i <= length}) 
-  (curr_heap:heap{forall j. {:pattern (Seq.index contents j)} 0 <= j /\ j < i ==> 
-    curr_heap.[addr + j] == UInt8.v (Seq.index contents j)}) : Lemma
-      (requires True)
-      (ensures (let new_heap = write_vale_mem contents length addr i curr_heap in
-      forall j. 0 <= j /\ j < length ==> UInt8.v (Seq.index contents j) == new_heap.[addr + j]))
-      (decreases %[sub length i])=
-      if i >= length then ()
-      else begin
-	let heap = curr_heap.[addr + i] <- UInt8.v (FStar.Seq.index contents i) in
-	load_store_write_vale_mem contents length addr (i+1) heap
-      end
-
-let rec domain_write_vale_mem 
-  (contents:Seq.seq UInt8.t) 
-  (length:nat{length = FStar.Seq.Base.length contents}) 
-  addr 
-  (i:nat{i <= length}) 
-  (curr_heap:heap{forall j. {:pattern (Seq.index contents j)} 0 <= j /\ j < i ==> 
-    curr_heap.[addr + j] == UInt8.v (Seq.index contents j)}) : Lemma
-      (requires True)
-      (ensures (let new_heap = write_vale_mem contents length addr i curr_heap in
-      forall j. Set.mem j (Map.domain new_heap) /\ not (Set.mem j (Map.domain curr_heap)) ==> 
-        addr <= j /\ j < addr + length))
-      (decreases %[sub length i])=
-   if i >= length then ()
-   else begin
-     let heap = curr_heap.[addr + i] <- UInt8.v (FStar.Seq.index contents i) in
-     domain_write_vale_mem contents length addr (i+1) heap
-    end
-
-let rec domain2_write_vale_mem 
-  (contents:Seq.seq UInt8.t) 
-  (length:nat{length = FStar.Seq.Base.length contents}) 
-  addr 
-  (i:nat{i <= length}) 
-  (curr_heap:heap{forall j. {:pattern (Seq.index contents j)} 0 <= j /\ j < i ==> 
-    curr_heap.[addr + j] == UInt8.v (Seq.index contents j)}) : Lemma
-      (requires forall j. addr <= j /\ j < addr + i ==> Set.mem j (Map.domain curr_heap))
-      (ensures (let new_heap = write_vale_mem contents length addr i curr_heap in
-	forall j. addr <= j /\ j < addr + length ==> Set.mem j (Map.domain new_heap)))
-      (decreases %[sub length i])=
-   if i >= length then ()
-   else begin
-     let heap = curr_heap.[addr + i] <- UInt8.v (FStar.Seq.index contents i) in
-     domain2_write_vale_mem contents length addr (i+1) heap
-    end
-
-let rec monotone_domain_write_vale_mem 
-  (contents:Seq.seq UInt8.t) 
-  (length:nat{length = FStar.Seq.Base.length contents}) 
-  addr 
-  (i:nat{i <= length}) 
-  (curr_heap:heap{forall j. {:pattern (Seq.index contents j)} 0 <= j /\ j < i ==> 
-    curr_heap.[addr + j] == UInt8.v (Seq.index contents j)}) : Lemma
-      (requires True)
-      (ensures (let new_heap = write_vale_mem contents length addr i curr_heap in
-      forall j. Set.mem j (Map.domain curr_heap) ==> Set.mem j (Map.domain new_heap)))
-      (decreases %[sub length i])=
-   if i >= length then ()
-   else begin
-     let heap = curr_heap.[addr + i] <- UInt8.v (FStar.Seq.index contents i) in
-     monotone_domain_write_vale_mem contents length addr (i+1) heap
-    end
-
-#set-options "--z3rlimit 40"
-
-let correct_down_p_cancel mem (addrs:addr_map) heap (p:b8) : Lemma
-  (forall p'. p == p' ==>       
-      (let length = B.length p in
-      let contents = B.as_seq mem p in
-      let addr = addrs p in
-      let new_heap = write_vale_mem contents length addr 0 heap in
-      correct_down_p mem addrs new_heap p')) = 
-  let rec aux (p':b8) : Lemma 
-    (p == p'  ==> (let length = B.length p in
-      let contents = B.as_seq mem p in
-      let addr = addrs p in
-      let new_heap = write_vale_mem contents length addr 0 heap in
-      correct_down_p mem addrs new_heap p')) =
-        let length = B.length p in
-        let contents = B.as_seq mem p in
-        let addr = addrs p in
-        let new_heap = write_vale_mem contents length addr 0 heap in
-	load_store_write_vale_mem contents length addr 0 heap
-  in
-  Classical.forall_intro aux
-      
-let correct_down_p_frame mem (addrs:addr_map) (heap:heap) (p:b8) : Lemma
-  (forall p'. disjoint p p' /\ correct_down_p mem addrs heap p' ==>       
-      (let length = B.length p in
-      let contents = B.as_seq mem p in
-      let addr = addrs p in
-      let new_heap = write_vale_mem contents length addr 0 heap in
-      correct_down_p mem addrs new_heap p')) = 
-  let rec aux (p':b8) : Lemma 
-    (disjoint p p' /\ correct_down_p mem addrs heap p' ==> (let length = B.length p in
-      let contents = B.as_seq mem p in
-      let addr = addrs p in
-      let new_heap = write_vale_mem contents length addr 0 heap in
-      correct_down_p mem addrs new_heap p')) =
-        let length = B.length p in
-        let contents = B.as_seq mem p in
-        let addr = addrs p in
-        let new_heap = write_vale_mem contents length addr 0 heap in
-	frame_write_vale_mem contents length addr 0 heap
-  in
-  Classical.forall_intro aux
-
-
-
-private let add_buffer_domain (b:b8) (addrs:addr_map) (accu:Set.set int) : GTot (s:Set.set int{
-  forall x. Set.mem x s <==> (Set.mem x accu \/ (x >= addrs b /\ x < addrs b + B.length b))}) =
-  let rec aux (j:nat{j <= B.length b}) (acc:Set.set int{forall x. Set.mem x acc <==>
+private let add_buffer_domain (b:buf) (addrs:addr_map) (accu:Set.set int) : GTot (s:Set.set int{
+  forall x. Set.mem x s <==> (Set.mem x accu \/ (x >= addrs b /\ x < addrs b + buf_length b))}) =
+  let rec aux (j:nat{j <= buf_length b}) (acc:Set.set int{forall x. Set.mem x acc <==>
     Set.mem x accu \/ (x >= addrs b /\ x < addrs b + j)}) :
     GTot (s:Set.set int{forall x. Set.mem x s <==>
-    Set.mem x accu \/ (x >= addrs b /\ x < addrs b + B.length b)}) 
-    (decreases %[B.length b - j]) = 
-    if j >= B.length b then acc else begin
+    Set.mem x accu \/ (x >= addrs b /\ x < addrs b + buf_length b)}) 
+    (decreases %[buf_length b - j]) = 
+    if j >= buf_length b then acc else begin
       let s = Set.union acc (Set.singleton (addrs b + j)) in
       aux (j+1) s
     end in
   aux 0 accu
   
 
-private let rec addrs_set_aux (ptrs:list b8)
-			      (ps2: list b8)
-			      (ps:list b8{forall b. List.memP b ptrs <==> List.memP b ps \/ List.memP b ps2})
-			      (addrs:addr_map)
-			      (accu:Set.set int{forall (x:int). not (Set.mem x accu) <==>
-			        (forall (b:b8{List.memP b ps}). x < addrs b \/ x >= addrs b + B.length b)}) :
-			 GTot (s:Set.set int{forall (x:int). not (Set.mem x s) <==>
-			        (forall (b:b8{List.memP b ptrs}). x < addrs b \/ x >= addrs b + B.length b)}) =
+private let rec addrs_set_aux
+  (ptrs:list buf)
+  (ps2: list buf)
+  (ps:list buf{forall b. List.memP b ptrs <==> List.memP b ps \/ List.memP b ps2})
+  (addrs:addr_map)
+  (accu:Set.set int{forall (x:int). not (Set.mem x accu) <==>
+    (forall (b:buf{List.memP b ps}). x < addrs b \/ x >= addrs b + buf_length b)}) :
+  GTot (s:Set.set int{forall (x:int). not (Set.mem x s) <==>
+    (forall (b:buf{List.memP b ptrs}). x < addrs b \/ x >= addrs b + buf_length b)}) =
   match ps2 with
   | [] -> accu
   | a::q -> 
@@ -190,8 +54,8 @@ private let rec addrs_set_aux (ptrs:list b8)
     let aux (x:int) : Lemma
       (requires True)
       (ensures not (Set.mem x s) <==> 
-      (forall (b:b8{List.memP b (a::ps)}). 
-	x < addrs b \/ x >= addrs b + B.length b)) = ()
+      (forall (b:buf{List.memP b (a::ps)}). 
+	x < addrs b \/ x >= addrs b + buf_length b)) = ()
     in
     Classical.forall_intro aux;
     addrs_set_aux ptrs q (a::ps) addrs s
@@ -211,42 +75,414 @@ let addrs_set_concat ptrs a addrs =
 
 let addrs_set_mem ptrs a addrs i = ()
 
-let write_buffer_vale (a:b8) (heap:heap) (mem:HS.mem) (addrs:addr_map) =
-  let length = B.length a in
-  let contents = B.as_seq mem a in
-  let addr = addrs a in
-  write_vale_mem contents length addr 0 heap
+(* Write a buffer in the vale memory *)
 
-let domain_write_buffer (a:b8) (heap:heap) (mem:HS.mem) (addrs:addr_map) : Lemma
-  (let new_heap = write_buffer_vale a heap mem addrs in
-   Set.equal (Set.union (Map.domain heap) (addrs_set [a] addrs)) (Map.domain new_heap)) =
-   let new_heap = write_buffer_vale a heap mem addrs in
-   let s1 = Map.domain heap in
-   let s2 = addrs_set [a] addrs in
-   let s3 = Map.domain new_heap in
-   let length = B.length a in
-   let contents = B.as_seq mem a in
-   let addr = addrs a in   
-   domain_write_vale_mem contents length addr 0 heap;
-   domain2_write_vale_mem contents length addr 0 heap;
-   monotone_domain_write_vale_mem contents length addr 0 heap;
-   ()
+let rec write_vale_mem8 (contents:Seq.seq UInt8.t) (length:nat{length = Seq.length contents}) addr (i:nat{i <= length}) 
+      (curr_heap:heap{forall j. {:pattern (Seq.index contents j)} 
+	0 <= j /\ j < i ==> curr_heap.[addr+j] == UInt8.v (Seq.index contents j)}) : Tot heap (decreases %[sub length i]) =
+    if i >= length then curr_heap
+    else (
+      let heap = curr_heap.[addr + i] <- UInt8.v (FStar.Seq.index contents i) in
+      write_vale_mem8 contents length addr (i+1) heap
+    )      
 
-let rec down_mem_aux (ptrs:list b8{list_disjoint_or_eq ptrs})
+let rec frame_write_vale_mem8 (contents:Seq.seq UInt8.t) (length:nat{length = FStar.Seq.Base.length contents}) addr (i:nat{i <= length}) 
+      (curr_heap:heap{forall j. {:pattern (Seq.index contents j)} 0 <= j /\ j < i ==> curr_heap.[addr + j] == UInt8.v (Seq.index contents j)}) : Lemma
+      (requires True)
+      (ensures (let new_heap = write_vale_mem8 contents length addr i curr_heap in
+      forall j. j < addr \/ j >= addr + length ==> curr_heap.[j] == new_heap.[j]))
+      (decreases %[sub length i])=
+      if i >= length then ()
+      else begin
+	let heap = curr_heap.[addr + i] <- UInt8.v (FStar.Seq.index contents i) in
+	frame_write_vale_mem8 contents length addr (i+1) heap
+      end
+      
+let rec load_store_write_vale_mem8
+  (contents:Seq.seq UInt8.t) 
+  (length:nat{length = FStar.Seq.Base.length contents}) 
+  addr 
+  (i:nat{i <= length}) 
+  (curr_heap:heap{forall j. {:pattern (Seq.index contents j)} 0 <= j /\ j < i ==> 
+    curr_heap.[addr + j] == UInt8.v (Seq.index contents j)}) : Lemma
+      (requires True)
+      (ensures (let new_heap = write_vale_mem8 contents length addr i curr_heap in
+      forall j. 0 <= j /\ j < length ==> UInt8.v (Seq.index contents j) == new_heap.[addr + j]))
+      (decreases %[sub length i])=
+      if i >= length then ()
+      else begin
+	let heap = curr_heap.[addr + i] <- UInt8.v (FStar.Seq.index contents i) in
+	load_store_write_vale_mem8 contents length addr (i+1) heap
+      end
+
+let rec domain_write_vale_mem8
+  (contents:Seq.seq UInt8.t) 
+  (length:nat{length = FStar.Seq.Base.length contents}) 
+  addr 
+  (i:nat{i <= length}) 
+  (curr_heap:heap{forall j. {:pattern (Seq.index contents j)} 0 <= j /\ j < i ==> 
+    curr_heap.[addr + j] == UInt8.v (Seq.index contents j)}) : Lemma
+      (requires True)
+      (ensures (let new_heap = write_vale_mem8 contents length addr i curr_heap in
+      forall j. Set.mem j (Map.domain new_heap) /\ not (Set.mem j (Map.domain curr_heap)) ==> 
+        addr <= j /\ j < addr + length))
+      (decreases %[sub length i])=
+   if i >= length then ()
+   else begin
+     let heap = curr_heap.[addr + i] <- UInt8.v (FStar.Seq.index contents i) in
+     domain_write_vale_mem8 contents length addr (i+1) heap
+    end
+
+let rec domain2_write_vale_mem8 
+  (contents:Seq.seq UInt8.t) 
+  (length:nat{length = FStar.Seq.Base.length contents}) 
+  addr 
+  (i:nat{i <= length}) 
+  (curr_heap:heap{forall j. {:pattern (Seq.index contents j)} 0 <= j /\ j < i ==> 
+    curr_heap.[addr + j] == UInt8.v (Seq.index contents j)}) : Lemma
+      (requires forall j. addr <= j /\ j < addr + i ==> Set.mem j (Map.domain curr_heap))
+      (ensures (let new_heap = write_vale_mem8 contents length addr i curr_heap in
+	forall j. addr <= j /\ j < addr + length ==> Set.mem j (Map.domain new_heap)))
+      (decreases %[sub length i])=
+   if i >= length then ()
+   else begin
+     let heap = curr_heap.[addr + i] <- UInt8.v (FStar.Seq.index contents i) in
+     domain2_write_vale_mem8 contents length addr (i+1) heap
+    end
+
+let rec monotone_domain_write_vale_mem8
+  (contents:Seq.seq UInt8.t) 
+  (length:nat{length = FStar.Seq.Base.length contents}) 
+  addr 
+  (i:nat{i <= length}) 
+  (curr_heap:heap{forall j. {:pattern (Seq.index contents j)} 0 <= j /\ j < i ==> 
+    curr_heap.[addr + j] == UInt8.v (Seq.index contents j)}) : Lemma
+      (requires True)
+      (ensures (let new_heap = write_vale_mem8 contents length addr i curr_heap in
+      forall j. Set.mem j (Map.domain curr_heap) ==> Set.mem j (Map.domain new_heap)))
+      (decreases %[sub length i])=
+   if i >= length then ()
+   else begin
+     let heap = curr_heap.[addr + i] <- UInt8.v (FStar.Seq.index contents i) in
+     monotone_domain_write_vale_mem8 contents length addr (i+1) heap
+    end
+
+#set-options "--z3rlimit 10"
+
+let rec write_vale_mem32 
+  (contents:Seq.seq UInt32.t) 
+  (length:nat{length = Seq.length contents}) 
+  addr
+  (i:nat{i <= length}) 
+  (curr_heap:heap{forall j. {:pattern (Seq.index contents j)} 0 <= j /\ j < i ==> 
+    (forall k. 0 <= k /\ k < 4 ==> 
+      curr_heap.[addr+ 4 `op_Multiply` j + k] == 
+      UInt8.v (Seq.index (put32_def (Seq.index contents j)) k))}) :
+  GTot heap (decreases %[sub length i]) =
+    if i >= length then curr_heap
+    else (
+      let put = put32_def (Seq.index contents i) in
+      let heap = curr_heap.[addr + 4 `op_Multiply` i + 0] <- UInt8.v (Seq.index put 0) in
+      let heap = heap.[addr + 4 `op_Multiply` i + 1] <- UInt8.v (Seq.index put 1) in
+      let heap = heap.[addr + 4 `op_Multiply` i + 2] <- UInt8.v (Seq.index put 2) in
+      let heap = heap.[addr + 4 `op_Multiply` i + 3] <- UInt8.v (Seq.index put 3) in      
+      write_vale_mem32 contents length addr (i+1) heap
+    )      
+
+let rec frame_write_vale_mem32
+  (contents:Seq.seq UInt32.t)
+  (length:nat{length = Seq.length contents}) 
+  addr 
+  (i:nat{i <= length}) 
+  (curr_heap:heap{forall j. {:pattern (Seq.index contents j)} 0 <= j /\ j < i ==>
+    (forall k. 0 <= k /\ k < 4 ==> 
+      curr_heap.[addr + 4 `op_Multiply` j + k] == 
+      UInt8.v (Seq.index (put32_def (Seq.index contents j)) k))}) : 
+  Lemma
+    (requires True)
+    (ensures (
+      let new_heap = write_vale_mem32 contents length addr i curr_heap in
+      forall j. j < addr \/ j >= addr + 4 `op_Multiply` length ==> curr_heap.[j] == new_heap.[j]))
+      (decreases %[sub length i]) =
+   if i >= length then ()
+   else begin
+      let put = put32_def (Seq.index contents i) in
+      let heap = curr_heap.[addr + 4 `op_Multiply` i + 0] <- UInt8.v (Seq.index put 0) in
+      let heap = heap.[addr + 4 `op_Multiply` i + 1] <- UInt8.v (Seq.index put 1) in
+      let heap = heap.[addr + 4 `op_Multiply` i + 2] <- UInt8.v (Seq.index put 2) in
+      let heap = heap.[addr + 4 `op_Multiply` i + 3] <- UInt8.v (Seq.index put 3) in  
+      frame_write_vale_mem32 contents length addr (i+1) heap
+   end
+      
+let rec load_store_write_vale_mem32 
+  (contents:Seq.seq UInt32.t) 
+  (length:nat{length = FStar.Seq.Base.length contents}) 
+  addr 
+  (i:nat{i <= length}) 
+  (curr_heap:heap{forall j. {:pattern (Seq.index contents j)} 0 <= j /\ j < i ==> 
+    (forall k. 0 <= k /\ k < 4 ==> 
+      curr_heap.[addr + 4 `op_Multiply` j + k] == 
+      UInt8.v (Seq.index (put32_def (Seq.index contents j)) k))}) : 
+  Lemma
+    (requires True)
+    (ensures (
+      let new_heap = write_vale_mem32 contents length addr i curr_heap in
+      forall j. 0 <= j /\ j < length ==>
+        (forall k. 0 <= k /\ k < 4 ==> 
+          new_heap.[addr + 4 `op_Multiply` j + k] == 
+          UInt8.v (Seq.index (put32_def (Seq.index contents j)) k))))
+      (decreases %[sub length i])=
+  if i >= length then ()
+  else begin
+    let put = put32_def (Seq.index contents i) in
+    let heap = curr_heap.[addr + 4 `op_Multiply` i + 0] <- UInt8.v (Seq.index put 0) in
+    let heap = heap.[addr + 4 `op_Multiply` i + 1] <- UInt8.v (Seq.index put 1) in
+    let heap = heap.[addr + 4 `op_Multiply` i + 2] <- UInt8.v (Seq.index put 2) in
+    let heap = heap.[addr + 4 `op_Multiply` i + 3] <- UInt8.v (Seq.index put 3) in  
+    load_store_write_vale_mem32 contents length addr (i+1) heap
+  end
+
+let rec domain_write_vale_mem32 
+  (contents:Seq.seq UInt32.t) 
+  (length:nat{length = Seq.length contents}) 
+  addr 
+  (i:nat{i <= length}) 
+  (curr_heap:heap{forall j. {:pattern (Seq.index contents j)} 0 <= j /\ j < i ==> 
+    (forall k. 0 <= k /\ k < 4 ==> 
+      curr_heap.[addr + 4 `op_Multiply` j + k] == 
+      UInt8.v (Seq.index (put32_def (Seq.index contents j)) k))}) : 
+  Lemma
+    (requires True)
+    (ensures (
+      let new_heap = write_vale_mem32 contents length addr i curr_heap in
+      forall j. Set.mem j (Map.domain new_heap) /\ not (Set.mem j (Map.domain curr_heap)) ==> 
+      addr <= j /\ j < addr + 4 `op_Multiply` length))
+      (decreases %[sub length i])=
+   if i >= length then ()
+   else begin
+    let put = put32_def (Seq.index contents i) in
+    let heap = curr_heap.[addr + 4 `op_Multiply` i + 0] <- UInt8.v (Seq.index put 0) in
+    let heap = heap.[addr + 4 `op_Multiply` i + 1] <- UInt8.v (Seq.index put 1) in
+    let heap = heap.[addr + 4 `op_Multiply` i + 2] <- UInt8.v (Seq.index put 2) in
+    let heap = heap.[addr + 4 `op_Multiply` i + 3] <- UInt8.v (Seq.index put 3) in  
+    domain_write_vale_mem32 contents length addr (i+1) heap
+  end
+
+let rec domain2_write_vale_mem32
+  (contents:Seq.seq UInt32.t) 
+  (length:nat{length = Seq.length contents}) 
+  addr 
+  (i:nat{i <= length}) 
+  (curr_heap:heap{forall j. {:pattern (Seq.index contents j)} 0 <= j /\ j < i ==> 
+    (forall k. 0 <= k /\ k < 4 ==> 
+      curr_heap.[addr + 4 `op_Multiply` j + k] == 
+      UInt8.v (Seq.index (put32_def (Seq.index contents j)) k))}) : 
+  Lemma
+    (requires forall j. addr <= j /\ j < addr + 4 `op_Multiply` i ==> Set.mem j (Map.domain curr_heap))
+    (ensures (  
+      let new_heap = write_vale_mem32 contents length addr i curr_heap in
+      forall j. addr <= j /\ j < addr + 4 `op_Multiply` length ==> Set.mem j (Map.domain new_heap)))
+      (decreases %[sub length i])=
+  if i >= length then ()
+  else begin
+    let put = put32_def (Seq.index contents i) in
+    let heap = curr_heap.[addr + 4 `op_Multiply` i + 0] <- UInt8.v (Seq.index put 0) in
+    let heap = heap.[addr + 4 `op_Multiply` i + 1] <- UInt8.v (Seq.index put 1) in
+    let heap = heap.[addr + 4 `op_Multiply` i + 2] <- UInt8.v (Seq.index put 2) in
+    let heap = heap.[addr + 4 `op_Multiply` i + 3] <- UInt8.v (Seq.index put 3) in  
+    domain2_write_vale_mem32 contents length addr (i+1) heap
+  end
+
+let rec monotone_domain_write_vale_mem32
+  (contents:Seq.seq UInt32.t) 
+  (length:nat{length = Seq.length contents}) 
+  addr 
+  (i:nat{i <= length}) 
+  (curr_heap:heap{forall j. {:pattern (Seq.index contents j)} 0 <= j /\ j < i ==> 
+    (forall k. 0 <= k /\ k < 4 ==> 
+      curr_heap.[addr + 4 `op_Multiply` j + k] == 
+      UInt8.v (Seq.index (put32_def (Seq.index contents j)) k))}) :
+  Lemma
+      (requires True)
+      (ensures (
+        let new_heap = write_vale_mem32 contents length addr i curr_heap in
+        forall j. Set.mem j (Map.domain curr_heap) ==> Set.mem j (Map.domain new_heap)))
+      (decreases %[sub length i])=
+  if i >= length then ()
+  else begin
+    let put = put32_def (Seq.index contents i) in
+    let heap = curr_heap.[addr + 4 `op_Multiply` i + 0] <- UInt8.v (Seq.index put 0) in
+    let heap = heap.[addr + 4 `op_Multiply` i + 1] <- UInt8.v (Seq.index put 1) in
+    let heap = heap.[addr + 4 `op_Multiply` i + 2] <- UInt8.v (Seq.index put 2) in
+    let heap = heap.[addr + 4 `op_Multiply` i + 3] <- UInt8.v (Seq.index put 3) in 
+    monotone_domain_write_vale_mem32 contents length addr (i+1) heap
+  end
+
+let write_buffer_vale (b:buf) (heap:heap) (mem:HS.mem) (addrs:addr_map) = match b with
+  | B8 a ->
+    let length = B.length a in
+    let contents = B.as_seq mem a in
+    let addr = addrs b in
+    write_vale_mem8 contents length addr 0 heap
+  | B32 a ->
+    let length = B.length a in
+    let contents = B.as_seq mem a in
+    let addr = addrs b in
+    write_vale_mem32 contents length addr 0 heap
+
+let frame_write_vale_mem
+  (b:buf)
+  (heap:heap)
+  (mem:HS.mem)
+  (addrs:addr_map) :
+  Lemma (
+    let new_heap = write_buffer_vale b heap mem addrs in
+    forall j. j < addrs b \/ j >= addrs b + buf_length b ==> heap.[j] == new_heap.[j]) =
+  match b with
+  | B8 a ->
+    let length = B.length a in
+    let contents = B.as_seq mem a in
+    let addr = addrs b in
+    frame_write_vale_mem8 contents length addr 0 heap
+  | B32 a ->
+    let length = B.length a in
+    let contents = B.as_seq mem a in
+    let addr = addrs b in
+    frame_write_vale_mem32 contents length addr 0 heap
+
+let domain_write_vale_mem
+  (b:buf)
+  (heap:heap)
+  (mem:HS.mem)
+  (addrs:addr_map) :
+  Lemma (
+    let new_heap = write_buffer_vale b heap mem addrs in
+    forall j. Set.mem j (Map.domain new_heap) /\ not (Set.mem j (Map.domain heap)) ==> 
+    addrs b <= j /\ j < addrs b + buf_length b) =
+  match b with
+  | B8 a ->
+    let length = B.length a in
+    let contents = B.as_seq mem a in
+    let addr = addrs b in
+    domain_write_vale_mem8 contents length addr 0 heap
+  | B32 a ->
+    let length = B.length a in
+    let contents = B.as_seq mem a in
+    let addr = addrs b in
+    domain_write_vale_mem32 contents length addr 0 heap
+
+let domain2_write_vale_mem
+  (b:buf)
+  (heap:heap)
+  (mem:HS.mem)
+  (addrs:addr_map) :
+  Lemma (
+    let new_heap = write_buffer_vale b heap mem addrs in
+    forall j. addrs b <= j /\ j < addrs b + buf_length b ==> Set.mem j (Map.domain new_heap)) =
+  match b with
+  | B8 a ->
+    let length = B.length a in
+    let contents = B.as_seq mem a in
+    let addr = addrs b in
+    domain2_write_vale_mem8 contents length addr 0 heap
+  | B32 a ->
+    let length = B.length a in
+    let contents = B.as_seq mem a in
+    let addr = addrs b in
+    domain2_write_vale_mem32 contents length addr 0 heap
+
+
+let monotone_domain_write_vale_mem
+  (b:buf)
+  (heap:heap)
+  (mem:HS.mem)
+  (addrs:addr_map) :
+  Lemma (
+    let new_heap = write_buffer_vale b heap mem addrs in
+    forall j. Set.mem j (Map.domain heap) ==> Set.mem j (Map.domain new_heap)) =
+  match b with
+  | B8 a ->
+    let length = B.length a in
+    let contents = B.as_seq mem a in
+    let addr = addrs b in
+    monotone_domain_write_vale_mem8 contents length addr 0 heap
+  | B32 a ->
+    let length = B.length a in
+    let contents = B.as_seq mem a in
+    let addr = addrs b in
+    monotone_domain_write_vale_mem32 contents length addr 0 heap
+
+let domain_write_buffer 
+  (a:buf) 
+  (heap:heap) 
+  (mem:HS.mem) 
+  (addrs:addr_map) :
+  Lemma
+    (let new_heap = write_buffer_vale a heap mem addrs in
+     Set.equal 
+       (Set.union (Map.domain heap) (addrs_set [a] addrs))
+       (Map.domain new_heap)) =
+   domain_write_vale_mem a heap mem addrs;
+   domain2_write_vale_mem a heap mem addrs;
+   monotone_domain_write_vale_mem a heap mem addrs
+
+let correct_down_p_cancel mem (addrs:addr_map) heap (p:buf) : Lemma
+  (forall p'. p == p' ==>       
+    (let new_heap = write_buffer_vale p heap mem addrs in
+    correct_down_p mem addrs new_heap p')) = 
+  let aux (p':buf) : Lemma 
+    (p == p' ==>
+      (let new_heap = write_buffer_vale p heap mem addrs in    
+      correct_down_p mem addrs new_heap p')) =
+      let new_heap = write_buffer_vale p heap mem addrs in
+        match p with
+        | B8 p ->
+          let length = B.length p in
+          let contents = B.as_seq mem p in
+          let addr = addrs (B8 p) in
+	  load_store_write_vale_mem8 contents length addr 0 heap
+        | B32 p ->
+          let length = B.length p in
+          let contents = B.as_seq mem p in
+          let addr = addrs (B32 p) in
+	  load_store_write_vale_mem32 contents length addr 0 heap
+  in
+  Classical.forall_intro aux
+      
+let correct_down_p_frame mem (addrs:addr_map) (heap:heap) (p:buf) : Lemma
+  (forall p'. disjoint p p' /\ correct_down_p mem addrs heap p' ==>       
+    (let new_heap = write_buffer_vale p heap mem addrs in
+    correct_down_p mem addrs new_heap p')) = 
+  let aux (p':buf) : Lemma 
+    (disjoint p p' /\ correct_down_p mem addrs heap p' ==> 
+      (let new_heap = write_buffer_vale p heap mem addrs in
+      correct_down_p mem addrs new_heap p')) =
+    let new_heap = write_buffer_vale p heap mem addrs in
+    match p with
+    | B8 p ->
+      let length = B.length p in
+      let contents = B.as_seq mem p in
+      let addr = addrs (B8 p) in
+      frame_write_vale_mem8 contents length addr 0 heap
+    | B32 p ->
+      let length = B.length p in
+      let contents = B.as_seq mem p in
+      let addr = addrs (B32 p) in
+      frame_write_vale_mem32 contents length addr 0 heap
+  in
+  Classical.forall_intro aux
+
+let rec down_mem_aux (ptrs:list buf{list_disjoint_or_eq ptrs})
   (addrs:addr_map)
   (mem:HS.mem)
-  (ps:list b8)
-  (accu:list b8{forall p. List.memP p ptrs <==> List.memP p ps \/ List.memP p accu})
+  (ps:list buf)
+  (accu:list buf{forall p. List.memP p ptrs <==> List.memP p ps \/ List.memP p accu})
   (h:heap{correct_down mem addrs accu h}) : 
   GTot (heap:heap{correct_down mem addrs ptrs heap}) =
   match ps with
     | [] -> addrs_set_lemma accu ptrs addrs; h
     | a::q ->
       let new_heap = write_buffer_vale a h mem addrs in
-      let length = B.length a in
-      let contents = B.as_seq mem a in
-      let addr = addrs a in      
-      load_store_write_vale_mem contents length addr 0 h;
       correct_down_p_cancel mem addrs h a;
       correct_down_p_frame mem addrs h a;
       assert (forall p. List.memP p accu ==> disjoint_or_eq p a);
@@ -261,32 +497,28 @@ let down_mem mem addrs ptrs =
   down_mem_aux ptrs addrs mem ptrs [] heap
 
 private
-let rec frame_down_mem_aux (ptrs:list b8{list_disjoint_or_eq ptrs})
+let rec frame_down_mem_aux (ptrs:list buf{list_disjoint_or_eq ptrs})
   (addrs:addr_map)
   (mem:HS.mem)
-  (ps:list b8)
-  (accu:list b8{forall p. List.memP p ptrs <==> List.memP p ps \/ List.memP p accu})
+  (ps:list buf)
+  (accu:list buf{forall p. List.memP p ptrs <==> List.memP p ps \/ List.memP p accu})
   (h:heap{correct_down mem addrs accu h}) : Lemma
   (let heap = down_mem_aux ptrs addrs mem ps accu h in
-   forall i. (forall (b:b8{List.memP b ptrs}). 
+   forall i. (forall (b:buf{List.memP b ptrs}). 
       let base = addrs b in
-      i < base \/ i >= base + B.length b) ==>
+      i < base \/ i >= base + buf_length b) ==>
       h.[i] == heap.[i]) =
   match ps with
   | [] -> ()
   | a::q ->
     let new_heap = write_buffer_vale a h mem addrs in
-    let length = B.length a in
-    let contents = B.as_seq mem a in
-    let addr = addrs a in     
-    load_store_write_vale_mem contents length addr 0 h;
     correct_down_p_cancel mem addrs h a;
     correct_down_p_frame mem addrs h a;
     assert (forall p. List.memP p accu ==> disjoint_or_eq p a);
     domain_write_buffer a h mem addrs;
     addrs_set_concat accu a addrs;    
     frame_down_mem_aux ptrs addrs mem q (a::accu) new_heap;
-    frame_write_vale_mem contents length addr 0 h;
+    frame_write_vale_mem a h mem addrs;
     ()
 
 let same_unspecified_down mem1 mem2 addrs ptrs =
@@ -298,37 +530,70 @@ let same_unspecified_down mem1 mem2 addrs ptrs =
   frame_down_mem_aux ptrs addrs mem2 ptrs [] heap;
   ()
 
-let get_seq_heap_as_seq (heap1 heap2:heap) (addrs:addr_map) (mem:HS.mem) (b:b8) : Lemma
+let buf_as_seq (mem:HS.mem) (b:buf) : GTot (if B8? b then Seq.seq UInt8.t else Seq.seq UInt32.t) = match b with
+  | B8 b -> B.as_seq mem b
+  | B32 b -> B.as_seq mem b
+
+#set-options "--z3rlimit 20"
+
+let get_seq_heap_as_seq 
+  (heap1 heap2:heap) 
+  (addrs:addr_map) 
+  (mem:HS.mem) 
+  (b:buf) : Lemma
   (requires correct_down_p mem addrs heap1 b /\
-    (forall x. x >= addrs b /\ x < addrs b + B.length b ==> heap1.[x] == heap2.[x]))
-  (ensures B.as_seq mem b == get_seq_heap heap2 addrs b) =
-  assert (Seq.equal (B.as_seq mem b) (get_seq_heap heap2 addrs b))
+    (forall x. x >= addrs b /\ x < addrs b + buf_length b ==> heap1.[x] == heap2.[x]))
+  (ensures buf_as_seq mem b == get_seq_heap heap2 addrs b) =
+  match b with
+  | B8 b ->
+    assert (Seq.equal (B.as_seq mem b) (get_seq_heap heap2 addrs (B8 b)))
+  | B32 a ->
+    reveal_opaque get32_def;
+    let seq_heap = get_seq_heap heap2 addrs b in
+    let aux (i:nat{i < B.length a}) =
+      // assume (Seq.index seq_heap i == UInt32.uint_to_t (
+      // heap2.[addrs b + 4 `op_Multiply` i + 0] +
+      // heap2.[addrs b + 4 `op_Multiply` i + 1] `op_Multiply` 0x100 +
+      // heap2.[addrs b + 4 `op_Multiply` i + 2] `op_Multiply` 0x10000 +
+      // heap2.[addrs b + 4 `op_Multiply` i + 3] `op_Multiply` 0x1000000));
+      ()
+
+      // let s2 = Seq.init 4 (fun (j:nat{j < 4}) -> heap2.[addrs (B32 b) + 4 `op_Multiply` i + j]) in
+      // assert (get32 s2 == Seq.index (get_seq_heap heap2 addrs (B32 b)) i)
+    in   
+    // assert (forall (i:nat{i < B.length b}). 
+    //   Seq.index (get_seq_heap heap2 addrs (B32 b)) i == 
+    //   get32 (Seq.init 4 (fun (j:nat{j < 4}) -> heap2.[addrs (B32 b) + 4 `op_Multiply` i + j])));
+    admit();
+    assert (Seq.equal (B.as_seq mem a) (get_seq_heap heap2 addrs b))
 
 let rec up_mem_aux (heap:heap)
                (addrs:addr_map)
-               (ptrs:list b8{list_disjoint_or_eq ptrs})
-               (ps:list b8)
-               (accu:list b8{forall p. List.memP p ptrs <==> List.memP p ps \/ List.memP p accu}) 
+               (ptrs:list buf{list_disjoint_or_eq ptrs})
+               (ps:list buf)
+               (accu:list buf{forall p. List.memP p ptrs <==> List.memP p ps \/ List.memP p accu}) 
                (m:HS.mem{list_live m ptrs /\ 
                  Set.equal (addrs_set ptrs addrs) (Map.domain heap) /\ 
                  (forall p. List.memP p accu ==> correct_down_p m addrs heap p)})
   : GTot (m':HS.mem{correct_down m' addrs ptrs heap /\ list_live m' ptrs}) =
     match ps with
     | [] -> m
-    | a::q ->
-      let s = get_seq_heap heap addrs a in
+    | (B8 a)::q ->
+      let s = get_seq_heap heap addrs (B8 a) in
       B.g_upd_seq_as_seq a s m;
       let m' = B.g_upd_seq a s m in
-      up_mem_aux heap addrs ptrs q (a::accu) m'
+      admit();
+      up_mem_aux heap addrs ptrs q ((B8 a)::accu) m'
+    | (B32 a)::q -> admit()
 
 let up_mem heap addrs ptrs mem = up_mem_aux heap addrs ptrs ptrs [] mem
 
 let rec down_up_identity_aux
     (heap:heap)
     (addrs:addr_map)
-    (ptrs:list b8{list_disjoint_or_eq ptrs})
-    (ps:list b8)
-    (accu:list b8{forall p. List.memP p ptrs <==> List.memP p ps \/ List.memP p accu})    
+    (ptrs:list buf{list_disjoint_or_eq ptrs})
+    (ps:list buf)
+    (accu:list buf{forall p. List.memP p ptrs <==> List.memP p ps \/ List.memP p accu})    
     (m:HS.mem{list_live m ptrs /\ correct_down m addrs ptrs heap})
   : Lemma (m == up_mem_aux heap addrs ptrs ps accu m) =
   match ps with
